work on Tseytin

theories/L/Complexity/Cook/FSAT_to_SAT.v
@@ -100,52 +100,277 @@ Hint Resolve varBound_cnf_monotonic.
 Hint Resolve varBound_cnf_app. 
 
 Hint Constructors varBound_cnf varBound_clause. 
-(*TODO: probably split up into compatibility lemmas for the different cases *)
-Lemma tseytin'_repr f nf v N nf' : varBound_formula nf f -> tseytin' nf f = (v, N, nf') -> varBound_cnf nf' N /\ v < nf' /\ formula_repr f N v. 
+
+(*for the proof of correctness, a stronger notion of representation is needed *)
+Definition assignment_lower_bound a n := forall v, v el a -> v >= n.
+Definition restrict a n := filter (fun v => v <? n) a.
+Definition join (a a' : assgn) := a ++ a'.
+
+Lemma assignment_lower_bound_app a1 a2 n: assignment_lower_bound (a1 ++ a2) n <-> assignment_lower_bound a1 n /\ assignment_lower_bound a2 n.
 Proof. 
-  revert nf nf' v N. induction f; cbn; intros. 
-  - inv H0. split; [ eauto | split; [lia | ]].
-    split; intros. 
-    + exists [v]; cbn. unfold satisfies. do 2 (cbn; rewrite Nat.eqb_refl). easy. 
-    + exists []; easy.
-  - inv H0. split; [eauto | split; [inv H; lia | ]]. split; intros [a H1]; exists a. 
-    + unfold FSAT.satisfies in H1. apply evalFormula_prim_iff in H1. unfold satisfies. cbn.
-      apply Bool.eqb_true_iff. now apply evalVar_in_iff. 
-    + unfold satisfies in H1. cbn in H1. apply Bool.eqb_prop in H1. apply evalVar_in_iff in H1. 
-      unfold FSAT.satisfies. now apply evalFormula_prim_iff. 
-  - destruct (tseytin' nf f1) as ((rv1 & N1) & nfVar1) eqn:F1.
-    destruct (tseytin' nfVar1 f2) as ((rv2 & N2) & nfVar2) eqn:F2. 
-    inv H. 
-    apply varBound_formula_monotonic with (n' := nf) in H3; [ | lia].
-    (*nfVar1 >= nf *)
-    specialize (tseytin'_nf_monotonic F1) as H7. 
-    specialize (tseytin'_nf_monotonic F2) as H8.
-    apply varBound_formula_monotonic with (n' := nfVar1) in H4; [ | lia].
-    specialize (IHf1 _ _ _ _ H3 F1) as (IH1 & IH2 & IH3).
-    specialize (IHf2 _ _ _ _ H4 F2) as (IH4 & IH5 & IH6).
-    inv H0. split; [ | split; [lia | ]].
-    + apply varBound_cnf_app; split; [ | apply varBound_cnf_app; split]; eauto 9.
-      eapply varBound_cnf_monotonic. 2: apply tseytinAnd_varBound. lia.
-    + split; intros [a H].
-      * exists (v :: rv1 :: rv2 :: a). unfold satisfies. 
-        unfold FSAT.satisfies in H; cbn in H. apply andb_true_iff in H as (He1 & He2).
-        (*better:app lemma *)
-        apply evalCnf_clause_iff. intros cl Hin. cbn in Hin. rewrite !in_app_iff in Hin. destruct_or Hin.
-        -- rewrite <- Hin. cbn. rewrite Nat.eqb_refl. easy.  
-        -- admit. (* use varBound to show that the new assignment is equivalent for the bounded cnf*)
-        -- admit. 
-        -- admit. 
-      * exists a. 
-        (*plan of attack: 
-          split along app/cons, derive that a[v] = true, use the equivalence for tseytinAnd, 
-          then the inductive hypotheses
-      *)
+  unfold assignment_lower_bound. setoid_rewrite in_app_iff. firstorder.
+Qed.
+
+Lemma assignment_lower_bound_monotonic a n n' : assignment_lower_bound a n -> n >= n' -> assignment_lower_bound a n'. 
+Proof. 
+  intros H H1. unfold assignment_lower_bound in *. intros v Hv; specialize (H v Hv); lia. 
+Qed. 
+
+Lemma evalVar_monotonic a a' v : a <<= a' -> evalVar a v = true -> evalVar a' v = true.
+Proof. 
+  intros H1 H2. rewrite evalVar_in_iff in *. firstorder.
+Qed. 
+
+Lemma evalLiteral_assgn_equiv a1 a2 l : a1 === a2 -> evalLiteral a1 l = evalLiteral a2 l. 
+Proof. 
+  intros [H1 H2]. destruct l as (b & v). unfold evalLiteral. destruct (evalVar a1 v) eqn:Hev1. 
+  - apply (evalVar_monotonic H1) in Hev1. easy.
+  - destruct (evalVar a2 v) eqn:Hev2; [ | easy]. 
+    apply (evalVar_monotonic H2) in Hev2. congruence. 
+Qed.
+
+Lemma evalClause_assgn_equiv a1 a2 c : a1 === a2 -> evalClause a1 c = evalClause a2 c. 
+Proof. 
+  intros H. enough (evalClause a1 c = true <-> evalClause a2 c = true).
+  - destruct evalClause; destruct evalClause; firstorder; easy. 
+  - rewrite !evalClause_literal_iff. now setoid_rewrite (evalLiteral_assgn_equiv _ H). 
+Qed.
+
+Lemma evalCnf_assgn_equiv a1 a2 c : a1 === a2 -> evalCnf a1 c = evalCnf a2 c. 
+Proof. 
+  intros H. enough (evalCnf a1 c = true <-> evalCnf a2 c = true). 
+  - destruct evalCnf; destruct evalCnf; firstorder; easy.
+  - rewrite !evalCnf_clause_iff. now setoid_rewrite (evalClause_assgn_equiv _ H).
+Qed. 
+
+Definition varInLiteral v (l : literal) := exists b, l = (b, v).
+Definition varInClause v c := exists l, l el c /\ varInLiteral v l. 
+Definition varInCnf v cn := exists cl, cl el cn /\ varInClause v cl. 
+
+
+Definition clause_varsIn (p : nat -> Prop) c := forall v, varInClause v c -> p v. 
+Definition cnf_varsIn (p : nat -> Prop) c := forall v, varInCnf v c -> p v. 
+
+Lemma clause_varsIn_varBound c n : clause_varsIn (fun v => v < n) c <-> varBound_clause n c. 
+Proof. 
+  induction c. 
+  - split; intros H; [eauto | intros v (? & [] &_)].
+  - split; intros H.
+    + destruct a as (b & v). econstructor.
+      * apply (H v). exists (b, v). split; [now left | exists b; easy].
+      * apply IHc. intros v' (l & H1). apply H. exists l. easy.
+    + inv H. apply IHc in H3. intros v (l & [<- | H4] & H5). 
+      * destruct H5 as (b' & H5). inv H5. lia. 
+      * apply H3. exists l. easy.
+Qed.
+
+Lemma cnf_varsIn_varBound c n: cnf_varsIn (fun v => v < n) c <-> varBound_cnf n c. 
+Proof. 
+  induction c. 
+  - split; intros H; [eauto | intros v (? & [] & _) ]. 
+  - split; intros H. 
+    + econstructor.
+      * apply clause_varsIn_varBound. intros v H1. apply H. exists a. easy. 
+      * apply IHc. intros v' (cl & H1). apply H. exists cl. easy.
+    + inv H. apply IHc in H3. apply clause_varsIn_varBound in H2. intros v (cl & [<- | H4] & H5). 
+      * apply (H2 v H5). 
+      * apply H3. exists cl. easy.
+Qed.
+
+(*it does not suffice to use formula_maxVar f instead of the parameter bound: the induction will fail 
+  as we have to show that formula_maxVar (f1 ∧ f2) is a lower bound...*)
+Definition tseytin_formula_repr (f : formula) (N : cnf) (v : var) (bound : nat):= 
+  (forall a, FSAT.satisfies a f -> exists a', assignment_lower_bound a' bound /\ SAT.satisfies (join a' a) ([(true, v)] :: N))
+  /\ (forall a, SAT.satisfies a ([(true, v)] :: N) -> FSAT.satisfies (restrict a (formula_maxVar f)) f). 
+
+Lemma join_extension_formula_equisat n f a a': varBound_formula n f -> assignment_lower_bound a' n -> (FSAT.satisfies a f <-> FSAT.satisfies (join a a') f).
+Proof. 
+  intros H H0.
+  unfold FSAT.satisfies. induction f. 
+  - cbn; tauto.
+  - rewrite !evalFormula_prim_iff. inv H. unfold assignment_lower_bound in H0.
+    unfold join.
+    split; [intros; now apply in_app_iff | ]. 
+    intros [H1 | H1]%in_app_iff; [easy | ].
+    apply H0 in H1. lia.  
+  - inv H. rewrite !evalFormula_and_iff. 
+    apply (varBound_formula_monotonic H5) in H3. 
+    apply (varBound_formula_monotonic H6) in H4.
+    apply IHf1 in H3. apply IHf2 in H4. 
+    tauto.
+  - inv H. rewrite !evalFormula_or_iff. 
+    apply (varBound_formula_monotonic H5) in H3. 
+    apply (varBound_formula_monotonic H6) in H4.
+    apply IHf1 in H3. apply IHf2 in H4. 
+    tauto.
+  - inv H. apply IHf in H2. rewrite !evalFormula_not_iff. tauto.
+Qed.
+
+
+(*an actually usable version of the lemma without useless bool2Prop stuff *)
+Lemma in_filter_iff (X : Type) (x : X) (p : X -> bool) (A : list X): x el filter p A <-> x el A /\ p x = true. 
+Proof. 
+  induction A; cbn. 
+  - tauto. 
+  - destruct (p a) eqn:H1.
+    + cbn. rewrite IHA. split; [intros [-> | [H2 H3]]; tauto | tauto ]. 
+    + rewrite IHA. split; [tauto | intros [[-> | H2] H3]; [congruence | tauto] ]. 
+Qed.
+
+Lemma restrict_formula_equisat n f a : varBound_formula n f -> (FSAT.satisfies a f <-> FSAT.satisfies (restrict a n) f). 
+Proof.
+  intros H. unfold FSAT.satisfies, restrict. induction f. 
+  - cbn; tauto.
+  - inv H. rewrite !evalFormula_prim_iff. rewrite in_filter_iff. 
+    rewrite Nat.ltb_lt. easy.
+  - inv H. rewrite !evalFormula_and_iff.
+    apply (varBound_formula_monotonic H4) in H2. 
+    apply (varBound_formula_monotonic H5) in H3.
+    apply IHf1 in H2. apply IHf2 in H3. tauto.
+  - inv H. rewrite !evalFormula_or_iff.
+    apply (varBound_formula_monotonic H4) in H2. 
+    apply (varBound_formula_monotonic H5) in H3.
+    apply IHf1 in H2. apply IHf2 in H3. tauto.  
+  - inv H. rewrite !evalFormula_not_iff.
+    apply IHf in H1. tauto.
+Qed.
+
+Fact app_singleton (X : Type) (x : X) (l : list X) : x::l = [x] ++ l. 
+Proof. easy. Qed.
+
+Lemma join_extension_cnf_monotonic a a' c : SAT.satisfies a c -> SAT.satisfies (join a' a) c. 
+Proof. 
+  (*intros H. unfold join. apply *)
 Admitted. 
+
+Lemma and_compat f1 f2 b: 
+  varBound_formula b f1 -> varBound_formula b f2 
+  -> (forall nf nf' v N, nf >= b -> tseytin' nf f1 = (v, N, nf') -> cnf_varsIn (fun n => n < b \/ (n >= nf /\ n < nf')) N /\ v < nf' /\ tseytin_formula_repr f1 N v nf)
+  -> (forall nf nf' v N, nf >= b -> tseytin' nf f2 = (v, N, nf') -> cnf_varsIn (fun n => n < b \/ (n >= nf /\ n < nf')) N /\ v < nf' /\ tseytin_formula_repr f2 N v nf)
+  -> forall nf nf' v N, nf >= b -> tseytin' nf (f1 ∧ f2) = (v, N, nf') -> cnf_varsIn (fun n => n < b \/ (n >= nf /\ n < nf')) N /\ v < nf' /\ tseytin_formula_repr (f1 ∧ f2) N v nf. 
+Proof. 
+  (*cbn. intros IHf1 IHf2 nf nf' v N H H0.*)
+  (*destruct (tseytin' nf f1) as ((rv1 & N1) & nfVar1) eqn:F1.*)
+  (*destruct (tseytin' nfVar1 f2) as ((rv2 & N2) & nfVar2) eqn:F2. *)
+  (*inv H. *)
+  (*specialize (@varBound_formula_monotonic f1 n1 nf ltac:(lia) H3) as H3'.*)
+  (*specialize (tseytin'_nf_monotonic F1) as H7. *)
+  (*specialize (tseytin'_nf_monotonic F2) as H8.*)
+  (*specialize (@varBound_formula_monotonic f2 n2 nfVar1 ltac:(lia) H4) as H4'.*)
+  (*specialize (IHf1 nf nfVar1 _ _  H3' F1) as (IH1 & IH3 & IH2 & (IH31 & IH32)).*)
+  (*specialize (IHf2 nfVar1 nfVar2 _ _ H4' F2) as (IH4 & IH6 & IH5 & (IH61 & IH62)).*)
+  (*symmetry in H0. inv H0. split; [ | split; [ | split; [lia | ]]].*)
+  (*- apply varBound_cnf_app; split; [ | apply varBound_cnf_app; split]; eauto 9.*)
+    (*eapply varBound_cnf_monotonic. 2: apply tseytinAnd_varBound. lia.*)
+  (*-  *)
+  (*- split; intros a H.*)
+    (*+ clear IH62 IH32. unfold FSAT.satisfies in H. apply evalFormula_and_iff in H as (He1 & He2).*)
+      (*specialize (IH31 _ He1) as (a1' & G1 & G2). *)
+      (*specialize (IH61 _ He2) as (a2' & G3 & G4).*)
+      (*exists (nfVar2 :: a2' ++ a1'). split.*)
+      (*1: { *)
+        (*replace (nfVar2 :: a2' ++a1') with ([nfVar2] ++ a2' ++ a1') by easy. rewrite !assignment_lower_bound_app. *)
+        (*repeat split; [ | eapply assignment_lower_bound_monotonic; [apply G3 | lia] | easy]. intros v' [<- | []]. lia.*)
+      (*} *)
+      (*unfold join. cbn. unfold satisfies.*)
+      (*rewrite app_singleton in G2, G4. apply evalCnf_app_iff in G2. apply evalCnf_app_iff in G4. *)
+      (*setoid_rewrite app_singleton at 2. repeat rewrite evalCnf_app_iff; repeat split.*)
+      (** cbn. rewrite Nat.eqb_refl. easy.*)
+      (** destruct G2 as (_ & G2). clear G4. *)
+        (*replace (nfVar2 :: (a2' ++ a1') ++ a) with (join (nfVar2 :: a2') (a1' ++ a)) by (unfold join; firstorder). *)
+        (*eapply (join_extension_cnf_monotonic). apply G2. *)
+      (** destruct G4 as (_ & G4). clear G2. *)
+        (*unfold join in G4. rewrite app_singleton.*)
+        (*enough (evalCnf ([nfVar2] ++ a1' ++ a2' ++ a) N2 = true). *)
+        (*{ rewrite <- H. eapply evalCnf_assgn_equiv. rewrite <- app_assoc. *)
+          (*split; intros x; rewrite !in_app_iff in *; intros Hx; destruct_or Hx; eauto. *)
+        (*} *)
+        (*replace ([nfVar2] ++ a1' ++ a2' ++a) with (join (nfVar2 :: a1') (a2' ++ a)) by (unfold join; firstorder).*)
+        (*eapply (join_extension_cnf_monotonic). apply G4. *)
+      (** apply tseytinAnd_sat. split; [intros _ | intros _; cbn; rewrite Nat.eqb_refl; easy]. *)
+        (*destruct G2 as (G2 & _). destruct G4 as (G4 & _). *)
+        (*cbn in G2, G4. rewrite Bool.eqb_true_iff in G2. rewrite Bool.eqb_true_iff in G4.*)
+        (*split; eapply evalVar_monotonic. *)
+        (*2: apply G2. 3: apply G4. *)
+        (*all: unfold join; rewrite <- app_assoc, app_singleton; intros x; rewrite !in_app_iff; intros Hx; destruct_or Hx; eauto. *)
+    (*+ clear IH61 IH31. *)
+      (*cbn. apply evalFormula_and_iff. split.*)
+      (** enough (FSAT.satisfies (restrict a (formula_maxVar f1)) f1). *)
+        (*{ apply restrict_formula_equisat. 1: { eapply varBound_formula_monotonic; [ | apply formula_bound_varBound]. lia. }*)
+          (*apply restrict_formula_equisat in H0; [easy | apply formula_bound_varBound]. *)
+        (*} *)
+        (*eapply IH32. rewrite app_singleton in H. unfold satisfies in H. rewrite !evalCnf_app_iff in H.*)
+        (*destruct H as (X1 & X2 & _ & X4). *)
+        (*cbn in X1. apply eqb_prop in X1.*)
+        (*apply tseytinAnd_sat in X4. apply X4 in X1 as (X1 & _).*)
+        (*unfold satisfies. rewrite app_singleton, evalCnf_app_iff. *)
+        (*split; [ cbn; now rewrite X1 | apply X2]. *)
+      (** enough (FSAT.satisfies (restrict a (formula_maxVar f2)) f2). *)
+        (*{ apply restrict_formula_equisat. 1: { eapply varBound_formula_monotonic; [ | apply formula_bound_varBound]. lia. }*)
+          (*apply restrict_formula_equisat in H0; [easy | apply formula_bound_varBound]. *)
+        (*} *)
+        (*eapply IH62. rewrite app_singleton in H. unfold satisfies in H. rewrite !evalCnf_app_iff in H.*)
+        (*destruct H as (X1 & _ & X3 & X4). *)
+        (*cbn in X1. apply eqb_prop in X1.*)
+        (*apply tseytinAnd_sat in X4. apply X4 in X1 as (_ & X1).*)
+        (*unfold satisfies. rewrite app_singleton, evalCnf_app_iff. *)
+        (*split; [ cbn; now rewrite X1 | apply X3]. *)
+(*Qed.*)
+Admitted. 
+
+(*Lemma or_compat f1 f2: *)
+  (*(forall nf nf' v N, varBound_formula nf f1 -> tseytin' nf f1 = (v, N, nf') -> varBound_cnf nf' N /\ v < nf' /\ tseytin_formula_repr f1 N v nf)*)
+  (*-> (forall nf nf' v N, varBound_formula nf f2 -> tseytin' nf f2 = (v, N, nf') -> varBound_cnf nf' N /\ v < nf' /\ tseytin_formula_repr f2 N v nf)*)
+  (*-> forall nf nf' v N, varBound_formula nf (f1 ∨ f2) -> tseytin' nf (f1 ∨ f2) = (v, N, nf') -> varBound_cnf nf' N /\ v < nf' /\ tseytin_formula_repr (f1 ∨ f2) N v nf. *)
+(*Proof. *)
+ 
+(*Admitted.  *)
+
+(*Lemma not_compat f: *)
+  (*(forall nf nf' v N, varBound_formula nf f -> tseytin' nf f = (v, N, nf') -> varBound_cnf nf' N /\ v < nf' /\ tseytin_formula_repr f N v nf)*)
+  (*-> forall nf nf' v N, varBound_formula nf (¬ f) -> tseytin' nf (¬ f) = (v, N, nf') -> varBound_cnf nf' N /\ v < nf' /\ tseytin_formula_repr (¬ f) N v nf. *)
+(*Proof. *)
+ 
+(*Admitted. *)
+       
+Lemma tseytin'_repr b f nf v N nf' : varBound_formula b f -> nf >= b -> tseytin' nf f = (v, N, nf') -> cnf_varsIn (fun n => n < b \/ (n >= nf /\ n < nf')) N /\ v < nf' /\ tseytin_formula_repr f N v nf. 
+Proof. 
+  intros H. revert nf nf' v N. induction f; intros. 
+  - inv H. cbn in H1. inv H1. split. 
+    1 : { intros v'. intros (c & [<- | []] & (l & [<- | []] & H)). destruct H as (? & H). inv H. lia. } 
+    split; [ lia | split; intros]. 
+    + exists [v]; cbn. split. 
+      * intros v' [-> | []]. lia.
+      *  unfold satisfies. do 2 (cbn; rewrite Nat.eqb_refl). easy. 
+    + easy.
+  - inv H. split. 
+    1: { cbn in H1. inv H1. intros v'. intros (c & [] & H). }
+    inv H1. split; [ lia | split].
+    + intros a H2. unfold FSAT.satisfies in H2. apply evalFormula_prim_iff in H2. unfold satisfies. 
+      exists []. cbn. split; [easy | ].
+      apply Bool.eqb_true_iff. now apply evalVar_in_iff. 
+    + intros a H1. unfold satisfies in H1. cbn in H1. apply Bool.eqb_prop in H1. apply evalVar_in_iff in H1. 
+      apply restrict_formula_equisat. 1: apply formula_bound_varBound.
+      apply evalFormula_prim_iff, H1.
+  - inv H. apply (varBound_formula_monotonic H6) in H4. apply (varBound_formula_monotonic H7) in H5. 
+    now apply (and_compat H4 H5  (IHf1 H4) (IHf2 H5)).
+  (*- now apply (or_compat IHf1 IHf2).*)
+  (*- now apply (not_compat IHf).*)
+Admitted. 
+
+Proposition tseytin_formula_repr_s f N v nf: tseytin_formula_repr f N v nf -> formula_repr f N v. 
+Proof. 
+  intros [H1 H2]. split.
+  - intros (a & H). apply H1 in H as (a' & _ & H). exists (join a' a). apply H. 
+  - intros (a & H). apply H2 in H. exists (restrict a (formula_maxVar f)). apply H. 
+Qed. 
 
 Lemma tseytin_repr f v N : tseytin f = (v, N) -> formula_repr f N v. 
 Proof. 
   unfold tseytin. destruct tseytin' as ((repVar & N1) & nfvar') eqn:H1.
-  intros H; inv H. eapply tseytin'_repr; [ | apply H1].
+  intros H; inv H. 
+  specialize (tseytin'_repr). 
+  eapply tseytin'_repr; [ | apply H1].
   apply formula_bound_varBound.
 Qed.
   
